updated relational spec, added valid inputs and simple Z_of_string

src/C_strtoimax/AbstractSpec.v
@@ -1,329 +1,224 @@
 Require Import StructTact.StructTactics.
 Require Import Core.Core Core.Notations Core.Tactics Core.PtrLemmas.
-Require Import Spec.
+Require Import Spec Lists.List.
 
 Import ListNotations.
+Open Scope Z.
 
-Local Open Scope ByteScope.
+Notation option_lift := RingMicromega.map_option.
 
-(* Abstract specification *)
-
-(* The most abstract level: Coq byte list and Z *)
-
-(* String is a byte list *)
 Definition string := list byte.
 
+(** * Memory read *)
+(* read [n] consecutive bytes from memory [m] starting at addres [a] *)
+Definition bytes_of_mem (m : mem) (a : addr) (n : Z) : option (string) :=
+  let '(b, ofs) := a in
+  (option_lift proj_bytes) (Mem.loadbytes m b (Ptrofs.unsigned ofs) n).
+
+Definition bytes_between (m : mem) (a1 a2 : addr) : option (string) :=
+  match distance m a1 a2 with
+  | Some n => bytes_of_mem m a1 (Z.of_nat n + 1%Z)
+  | None => None
+  end.
+
+(** * High level spec *)
+(* common bytes *)
 Definition minus_char := Byte.repr 45.
 Definition plus_char := Byte.repr 43.
 Definition zero_char := Byte.repr 48.
+Definition nine_char := Byte.repr 57.
 
-Definition is_digit (i : byte) := (Byte.repr 48 <= i) && (i <= Byte.repr 57).
+Definition is_digit (i : byte) : bool :=
+  ((zero_char <= i) && (i <= nine_char))%byte.
 
-Section ZSpec.
+Definition Z_of_char (b : byte) : Z :=
+  Byte.signed b - Byte.signed zero_char.
 
-  (* Take a string s and return a pair with its integer representation *)
+Definition is_sign (b : byte) : bool :=
+  ((b == plus_char) || (b == minus_char))%byte.
 
-Definition string_to_Z (s : string) : option Z :=
-  let fix string_to_Z_loop s v :=
+Definition sign_of_char (b : byte) : Z :=
+  if (b == plus_char)%byte then 1
+  else if (b == minus_char)%byte then (- 1)
+       else 0.
+
+Definition bounded (n : Z) : bool :=
+  (Int.min_signed <=? n) && (n <=? Int.max_signed).
+
+(* s is not empty *)
+Definition non_empty (s : string) := s <> [].
+
+(* all characters in s are digits *)
+Definition all_digits (s : string) := forallb is_digit s.
+
+(* Valid inputs that can be successfully converted into int *)
+
+Inductive valid_input : string -> Prop :=
+| ValidInput_EXTRA_DATA : forall s' s,
+    (* s' represents a number (optionally) preceded by + or - *) 
+    valid_input_all_digits s' ->
+    (* append any string to s' to get extra data case *)
+    valid_input (app s' s)              
+with valid_input_all_digits : string -> Prop :=       
+     | ValidInput_OK_unsigned :
+         forall s,
+           non_empty s ->
+           all_digits s = true ->
+           valid_input_all_digits s
+     | ValidInput_OK_signed :
+         forall sg s,
+           non_empty s ->
+           is_sign sg = true ->
+           all_digits s = true ->
+           valid_input_all_digits (sg :: s).
+
+(* Converts string into an integer:
+   - returns None on empty string
+   - otherwise converts s into int until a non-digit is encountered 
+   - on [c], with c not a digit, returns 0 
+     (later we will call it only on valid data so this is irrelevant)  
+   - records index where extra data is encountered or where we go out of range *)
+
+Record Z_of_string_result :=
+  { val : Z ;
+    index : Z ;
+  }.
+
+Definition Z_of_string (sign : byte) (s : string) : option Z_of_string_result :=
+  let fix Z_of_string_loop s v i :=
       match s with
-      | [] => v
+      | [] => {| val := v ;
+                index := i ; |}
       | c :: tl =>
+        let i' := (Zlength s - (Zlength tl) - 1)%Z in (* index of c in s *)
         if is_digit c
         then let v := (v * 10 + (Byte.signed c - 48))%Z in
-             string_to_Z_loop tl v                
-        else v(* extra stuff is ignored *)     
+             if bounded v
+             then Z_of_string_loop tl v i
+             else Z_of_string_loop tl v i' (* recoreded where went out of range *)          
+        else {| val := v ;
+                index := i' ; |} (* extra stuff is ignored *)               
       end
   in match s with
-     | nil => None (* not enough data *)
-     | _ => Some (string_to_Z_loop s 0%Z)
-     end.
+     |  nil => None (* no data to convert *)
+     |  _ => let res := (Z_of_string_loop s 0%Z 0%Z) in
+            if (sign == plus_char)%byte
+            then Some res
+            else Some {| val := Z.opp (val res);
+                         index := index res ; |}
+                         end.
 
-(* The sign is determined by the first char in the string *)
-Definition signed_string_to_Z (s : string) :=
-  match s with
-  | nil => None 
-  | c :: tl => if c == minus_char
-             then option_map Z.opp (string_to_Z tl)      
-               else if c == plus_char
-                    then string_to_Z tl
-                    else string_to_Z s
-  end.
+(** Relational spec *)
+
+(* Store pointer (a2 + i) at address a1 *)
+Definition store_pointer (m : mem) (a1 : addr) (a2 : addr) (i : Z) :=
+  let (b1, ofs1) := a1 in
+  let (b2, ofs2) := a2 in
+  Mem.storev Mptr m (Vptr b1 ofs1) (Vptr b2 (ofs2 + (Ptrofs.repr i))%ptrofs).
+
+(* Store v as a long value at address a *)
+Definition store_value (m : mem) (a : addr) (v : Z) :=
+  let (b, ofs) := a in
+  Mem.storev Mint64 m (Vptr b ofs) (Vlong (Int64.repr v)).
+
+Inductive asn_strtoimax_lim_R m str fin intp : mem -> asn_strtox_result_e -> Prop :=
   
+(* Input outside of supported numeric range, first read sign *)
+| ASN_STRTOX_ERROR_RANGE_R_signed :
+    forall sg s z m',
+      bytes_between m str fin = Some (sg :: s) ->
+      is_sign sg = true ->
+      valid_input (sg :: s) ->
+      Z_of_string sg s = Some z ->
+      bounded (val z) = false ->
+      store_pointer m fin str (index z) = Some m' -> 
+      asn_strtoimax_lim_R m str fin intp m' ASN_STRTOX_ERROR_RANGE
+                          
+(* Input outside of supported numeric range *)
+| ASN_STRTOX_ERROR_RANGE_R_unsigned :
+    forall s z m',
+      bytes_between m str fin = Some s ->
+      valid_input s -> 
+      Z_of_string plus_char s = Some z ->
+      bounded (val z) = false ->
+      store_pointer m fin str (index z) = Some m' -> 
+      asn_strtoimax_lim_R m str fin intp m' ASN_STRTOX_ERROR_RANGE
 
-End ZSpec.
-
-
-
-Section RelationalSpec.
-
-  (* To relate the abstract spec we need to add assumption about memory *)
-Definition byte_of_int b := Byte.repr (Int.unsigned b).
-
-(* There is a string s at address str until fin *)
-(* Note: load returns value of type Vint, hence need a conversion from byte *)
-Definition string_at_address m str fin : option (list byte) :=
-  match load_addr Mptr m fin with
-    | Some (Vptr b fin') => 
-      match distance m str (b,fin') with
-      | Some dist =>
-        let fix string_at_address m s str dist : option (list byte) :=
-            match dist with
-            | O => Some s
-            | S n => match load_addr Mint8signed m str with
-                    | Some (Vint i) =>
-                      string_at_address m ((byte_of_int i)::s) (str++) n
-                    | _ => None
-                    end
-            end in
-        string_at_address m nil str dist
-      | _ => None
-      end
-    | _ => None
-  end.
-
-  (* Relational spec without memory stores *)
-  
-  Inductive asn_strtoimax_lim_R m str fin : asn_strtox_result_e -> Prop :=
-    (* Input outside of supported numeric range *)
-  | ASN_STRTOX_ERROR_RANGE_R s z :
-      string_at_address m str fin = Some s ->
-      signed_string_to_Z s = Some z ->
-      (Int64.max_signed <= z)%Z \/ (z <= Int64.min_signed)%Z ->
-      asn_strtoimax_lim_R m str fin ASN_STRTOX_ERROR_RANGE
-    (* Invalid data encountered (e.g., "+-") *)
-  | ASN_STRTOX_ERROR_INVAL_R :
-      addr_ge m str fin = Some true ->
-      asn_strtoimax_lim_R m str fin ASN_STRTOX_ERROR_INVAL
-    (* More data expected (e.g. "+") *)
-  | ASN_STRTOX_EXPECT_MORE_R :
-      string_at_address m str fin = Some [plus_char] \/
-      string_at_address m str fin = Some [minus_char] ->
-      asn_strtoimax_lim_R m str fin ASN_STRTOX_EXPECT_MORE
-    (* Conversion succeded, but the string has extra stuff *)
-  | ASN_STRTOX_EXTRA_DATA_R s z :
-      string_at_address m str fin = Some s ->
-      signed_string_to_Z s = Some z ->
-      (Int64.min_signed <= z <= Int64.max_signed)%Z ->
+(* Invalid data encountered (e.g., "+-", "a") *)                       
+| ASN_STRTOX_ERROR_INVAL_R_Some :
+    forall s,
+      bytes_between m str fin = Some s ->
+      ~ (valid_input s) ->
+      asn_strtoimax_lim_R m str fin intp m ASN_STRTOX_ERROR_INVAL
+                          
+(* str >= * end and memory fail (could replace by just str >= *end *)                          
+| ASN_STRTOX_ERROR_INVAL_R_None :
+    bytes_between m str fin = None ->
+    asn_strtoimax_lim_R m str fin intp m ASN_STRTOX_ERROR_INVAL
+                        
+(* More data expected (e.g. "+", "-") *)
+| ASN_STRTOX_EXPECT_MORE_R : forall m',
+    bytes_between m str fin = Some [plus_char] \/
+    bytes_between m str fin = Some [minus_char] ->
+    store_pointer m fin str 1%Z = Some m' ->
+    asn_strtoimax_lim_R m str fin intp m' ASN_STRTOX_EXPECT_MORE
+                        
+(* Conversion succeded, but the string has extra stuff, first read sign *)
+| ASN_STRTOX_EXTRA_DATA_R_signed :
+    forall sg s z m' m'',
+      bytes_between m str fin = Some (sg :: s) ->
+      valid_input (sg :: s) ->
       (exists c, In c s /\ is_digit c = false) ->
-      asn_strtoimax_lim_R m str fin ASN_STRTOX_EXTRA_DATA
-      (* Conversion succeded *)
-  | ASN_STRTOX_OK_R s z :
-      string_at_address m str fin = Some s ->
-      signed_string_to_Z s = Some z ->
-      (Int64.min_signed <= z <= Int64.max_signed)%Z ->
-      asn_strtoimax_lim_R m str fin ASN_STRTOX_OK.  
+      is_sign sg = true ->      
+      Z_of_string sg s = Some z ->
+      bounded (val z) = true ->
+      store_pointer m fin str (index z) = Some m' ->
+      store_value m' intp (val z) = Some m'' ->
+      asn_strtoimax_lim_R m str fin intp m'' ASN_STRTOX_EXTRA_DATA
 
-  (* Relational spec with memory stores *)
-  
-  (* We need to store a pointer where we stop in error range, extra data and ok case,
-     hence this additional function:
-
-     Take a string s and an index where either the first non-digit is encountered 
-     or we go out of range. If none of the above happens return (length s) *)
-
-Definition string_to_Z_endpoint (s : string) : option Z :=
-  let fix string_to_Z_loop s v z :=
-      match s with
-      | [] => z
-      | c :: tl =>
-        (* index of c in s *)
-        let i := (Zlength s - (Zlength tl) - 1)%Z in
-        if is_digit c
-        then let v := (v * 10 + (Byte.signed c - 48))%Z in
-             if (Int64.max_signed <=? z)%Z || (z <=? Int64.min_signed)%Z
-             then i
-             else string_to_Z_loop tl v z               
-        else i 
-      end
-  in match s with
-     | nil => None 
-     | _ => Some (string_to_Z_loop s 0%Z (Zlength s))
-     end.
-
-(* The sign is determined by the first char in the string *)
-Definition signed_string_to_Z_endpoint (s : string) :=
-  match s with
-  | nil => None 
-  | c :: tl => if (c == minus_char) || (c == plus_char)
-             then string_to_Z_endpoint tl     
-             else string_to_Z_endpoint s
-  end.
-  
-  Inductive asn_strtoimax_lim_R_mem m str fin intp : mem -> asn_strtox_result_e -> Prop :=
-    (* Input outside of supported numeric range *)
-  | ASN_STRTOX_ERROR_RANGE_R_mem s z m' i :
-      string_at_address m str fin = Some s ->
-      signed_string_to_Z s = Some z ->
-      signed_string_to_Z_endpoint s = Some i ->
-      (Int64.max_signed <= z)%Z \/ (z <= Int64.min_signed)%Z ->
-      store_addr Mptr m fin (vptr (add_addr str (Ptrofs.repr i)))
-      = Some m' -> 
-      asn_strtoimax_lim_R_mem m str fin intp m' ASN_STRTOX_ERROR_RANGE
-    (* Invalid data encountered (e.g., "+-") *)
-  | ASN_STRTOX_ERROR_INVAL_R_mem :
-      addr_ge m str fin = Some true ->
-      asn_strtoimax_lim_R_mem m str fin intp m ASN_STRTOX_ERROR_INVAL
-    (* More data expected (e.g. "+") *)
-  | ASN_STRTOX_EXPECT_MORE_R_mem m':
-      string_at_address m str fin = Some [plus_char] \/
-      string_at_address m str fin = Some [minus_char] ->
-      store_addr Mptr m fin (vptr (str++)) = Some m' -> 
-      asn_strtoimax_lim_R_mem m str fin intp m' ASN_STRTOX_EXPECT_MORE
-    (* Conversion succeded, but the string has extra stuff *)
-  | ASN_STRTOX_EXTRA_DATA_R_mem s z m' m'' i:
-      string_at_address m str fin = Some s ->
-      signed_string_to_Z s = Some z ->
-      signed_string_to_Z_endpoint s = Some i ->
-      (Int64.min_signed <= z <= Int64.max_signed)%Z ->
+(* Conversion succeded, but the string has extra stuff *)                          
+| ASN_STRTOX_EXTRA_DATA_R_unsigned :
+    forall s z m' m'',
+      bytes_between m str fin = Some s ->
+      valid_input s ->
       (exists c, In c s /\ is_digit c = false) ->
-      store_addr Mptr m fin (vptr (add_addr str (Ptrofs.repr i)))
-      = Some m' -> 
-      store_addr Mint64 m' intp (Vlong (Int64.repr z)) = Some m'' -> 
-      asn_strtoimax_lim_R_mem m str fin intp m'' ASN_STRTOX_EXTRA_DATA
-      (* Conversion succeded *)
-  | ASN_STRTOX_OK_R_mem s z m' m'':
-      string_at_address m str fin = Some s ->
-      signed_string_to_Z s = Some z ->
-      (Int64.min_signed <= z <= Int64.max_signed)%Z ->
-      store_addr Mptr m fin (vptr (add_addr str (Ptrofs.repr (Zlength s))))
-      = Some m' -> 
-      store_addr Mint64 m' intp (Vlong (Int64.repr z)) = Some m'' -> 
-      asn_strtoimax_lim_R_mem m str fin intp m'' ASN_STRTOX_OK.
-  
-End RelationalSpec.
+      Z_of_string plus_char s = Some z ->
+      bounded (val z) = true ->
+      store_pointer m fin str (index z) = Some m' ->
+      store_value m' intp (val z) = Some m'' ->
+      asn_strtoimax_lim_R m str fin intp m'' ASN_STRTOX_EXTRA_DATA
+                          
+(* Conversion succeded, first read sign *)
+| ASN_STRTOX_OK_R_signed :
+    forall sg s z m' m'',
+      bytes_between m str fin = Some (sg :: s) ->
+      is_sign sg = true ->
+      valid_input_all_digits (sg :: s) ->
+      Z_of_string sg s  = Some z ->
+      bounded (val z) = true ->
+      store_pointer m fin str (Zlength (sg :: s)) = Some m' ->
+      store_value m' intp (val z) = Some m'' ->
+      asn_strtoimax_lim_R m str fin intp m'' ASN_STRTOX_OK
 
-Theorem asn_strtoimax_lim_func_correct : forall m str fin fin' intp res val p s' m',
+| ASN_STRTOX_OK_R_unsigned :
+    forall s z m' m'',
+      bytes_between m str fin = Some s ->
+      valid_input_all_digits s ->
+      Z_of_string plus_char s = Some z ->
+      bounded (val z) = true ->
+      store_pointer m fin str (Zlength s) = Some m' ->
+      store_value m' intp (val z) = Some m'' ->
+      asn_strtoimax_lim_R m str fin intp m'' ASN_STRTOX_OK.                    
+                        
+Theorem asn_strtoimax_lim_func_correct : forall m str fin intp res val p s' m',
     asn_strtoimax_lim m str fin intp = Some {| return_type := res;
                                                value := val;
                                                str_pointer := p;
                                                memory := Some m';
                                                sign := s';|}
-    <-> asn_strtoimax_lim_R_mem m str fin' intp m' res.
-Proof.
-  intros.
-  split; intro.
-  induction res.
-  - econstructor.
-    all: admit.
-  - inversion H.
-    unfold string_at_address in *.
-    unfold signed_string_to_Z in *.
-    unfold asn_strtoimax_lim in *.
-    unfold store_result in *.
-    unfold distance in *.
-    unfold vptr in *.
-    repeat break_match; try congruence.
-    unfold addr_ge, ptr_ge in *.
-    Admitted.
+    <-> asn_strtoimax_lim_R m str fin intp m' res.
+Admitted.
     
-    
-(* Functional spec continued *)
-
-(* Moving towards implementation. Step 1: bounds on Z *)
-Section ZBoundsSpec.
-
-(* Assume some intsize and 2-complement encoding of negative int *)  
-Variable intsize : Z.
-Definition upper_boundZ := (intsize / 10)%Z.
-Definition last_digit_plusZ := (Zmod intsize 10)%Z.
-Definition last_digit_minusZ := (last_digit_plusZ + 1)%Z.
- 
-Definition string_to_Z_bound s last_digit :=
-  let fix string_to_Z_loop s v last_digit :=
-      match s with
-      | [] => Some v
-      | c :: tl =>
-        if is_digit c then
-          let d := (Byte.signed c - 48)%Z in
-          if (v <? upper_boundZ)%Z ||
-            ((v =? upper_boundZ)%Z && (d <=? last_digit)%Z)
-          then string_to_Z_loop tl (v * 10 + d)%Z
-                                last_digit
-          else None (* out of range *)
-        else Some v (* extra stuff is ignored *)     
-      end
-  in match s with
-     | nil => None (* empty string corresponds to nothing *)
-     | _ => (string_to_Z_loop s 0%Z last_digit)
-     end.
-
-(* The sign is determined by the first char in the string *)
-Definition signed_string_to_Z_bound s :=
-  match s with
-  | nil => None 
-  | c :: tl => if c == minus_char
-               then option_map
-                      Z.opp (string_to_Z_bound tl last_digit_minusZ)
-               else if c == plus_char
-                    then string_to_Z_bound tl last_digit_plusZ
-                    else string_to_Z_bound s last_digit_plusZ
-  end.
-
-End ZBoundsSpec.
-
-Section IntSpec.
-  
-Local Open Scope Int64Scope.
-
-(* Then we can formulate it on int *)
-Definition long_of_byte b := Int64.repr (Byte.unsigned b).
-
-Definition intmax := (Int64.repr Int64.max_unsigned).
-Definition upper_bound := Int64.repr (upper_boundZ Int64.max_unsigned).
-Definition lower_bound := Int64.neg upper_bound.
-Definition last_digit_plus := intmax % (Int64.repr 10).
-Definition last_digit_minus := (intmax % (Int64.repr 10)) + 1.
-
-Definition string_to_int_plus s :=
-  let fix string_to_Z_loop s v :=
-      match s with
-      | [] => Some v
-      | c :: tl =>
-        if is_digit c then
-          let d := (long_of_byte c - (Int64.repr 48)) in
-          if (v < upper_bound) ||
-             ((v == upper_bound) && (d <= last_digit_plus))
-          then
-            string_to_Z_loop tl (v * (Int64.repr 10) + d)
-          else None 
-        else Some v  
-      end
-  in match s with
-     | nil => None 
-     | _ => string_to_Z_loop s 0%int64
-     end.
-
-Definition string_to_int_minus s :=
-  let fix string_to_Z_loop s v :=
-      match s with
-      | [] => Some v
-      | c :: tl =>
-        if is_digit c then
-          let d := (long_of_byte c - (Int64.repr 48)) in
-          if (lower_bound < v) ||
-             ((v == lower_bound) && (d <= last_digit_minus))
-          then
-            string_to_Z_loop tl (v * (Int64.repr 10) - d)
-          else None 
-        else Some v  
-      end
-  in match s with
-     | nil => None 
-     | _ => string_to_Z_loop s 0%int64
-     end.
-
-(* The sign is determined by the first char in the string *)
-Definition signed_string_to_int s :=
-  match s with
-  | nil => None 
-  | c :: tl => if (c == minus_char)%byte
-               then string_to_int_minus tl
-               else if (c == plus_char)%byte
-                    then string_to_int_plus tl
-                    else string_to_int_plus s 
-  end.
-
-End IntSpec.
 
 
     
